theories/simpl.v
@@ -1,0 +1,37 @@
+From mathcomp Require Import all_ssreflect.
+From det Require Import zify_ssreflect.
+
+Inductive tree A :=
+  | E
+  | N : A -> tree A -> tree A -> tree A .
+
+Arguments N {_}.
+Arguments E {_}.
+
+Fixpoint f acc (l: tree nat) :=
+  match l with
+  | E => acc
+  | N v L R => 
+    f (acc + f v L) R
+  end.
+
+Fixpoint f1 (l: tree nat) :=
+  match l with
+  | E => 0
+  | N v L R => 
+    v + f1 L + f1 R
+  end.
+
+Definition T := N 3 (N 2 E E) E.
+Compute (f 0 T).
+Compute (f1 T).
+
+
+Lemma sum:
+  forall t n, f n t = n + f1 t.
+Proof.
+  elim => //=.
+  - lia.
+  - move=> hd l hl r hr n.
+    rewrite hr hl; lia.
+Qed.
